Add list select to rng
Also spec (but don't prove) boundary props of
rand_nat.

tryf/Quint.Rng.fst
@@ -1,6 +1,7 @@
 module Quint.Rng
 
 open FStar.Mul
+module List = FStar.List.Tot
 
 // An RNG adapted from https://raw.githubusercontent.com/informalsystems/quint/main/quint/src/rng.ts
 // with all the shortcomings and basis of that impl
@@ -15,7 +16,7 @@ let u64 = 0x10000000000000000
 
 let key = 0xfb9e125878fa6cb3
 
-let squares64 (s:state): int =
+let squares64 (s:state): nat =
   let x = (s.v * key) % u64 in
   let y = x in
   let z = (y + key) % u64 in
@@ -29,6 +30,7 @@ let squares64 (s:state): int =
   let x = (x / u32 + ((x * u32) % u64)) % u64 in
   // round 4
   ((((x * x) % u64) + z) % u64) / u32
+
 
 let rec rand_aux (s : state) (input:nat{input > 0}) (output base:int)
   : Tot (int & state)
@@ -46,9 +48,6 @@ let rec rand_aux (s : state) (input:nat{input > 0}) (output base:int)
     let state' = Rn ((s.v + 1) % u64) in
     output', state'
 
-let init (s:nat): state = Rn (s % u64)
-let rand (bound:nat{bound > 0}) : t int =
-  fun state -> rand_aux state bound 0 1
 
 let return #a (x:a): t a = fun s -> (x, s)
 
@@ -57,27 +56,77 @@ let (let?) #a #b (rng:t a) (f: a -> t b): t b=
     let r, s' = rng s in
     (f r) s'
 
+let init (s:nat): state = Rn (s % u64)
+
+// TODO: Prove boundary property
+/// [rand_int n] is a random nat `i` `0 <= i < n`
+let rand_nat (bound:nat{bound  > 0}): t (n:nat{n >= 0 /\ n < bound}) =
+  fun state ->
+  let n, s = rand_aux state bound 0 1 in
+  // XXX Bounds property is unproven! (But we know it holds)
+  assume (n >= 0 /\ n < bound);
+  n, s
+
+let rand_bool : t bool =
+  let? n = rand_nat 2 in
+  return (
+     if n < 1 then true else false
+  )
+
+let rand_choice #a (l : list a{List.length l > 0}) : t a =
+  let len = List.length l in
+  let? idx = rand_nat len in
+  // XXX Bounds property is unproven! (But we know it holds)
+  assume (idx >= 0 /\ idx < len);
+  return (List.index l idx)
+
 let run #a (s:state) (f:t a): a =
   let r, _ = f s in
   r
 
-let _ex1 =
+let _ex_rand_nat =
   let cmp =
-    let? w = rand 2 in
-    let? x = rand 2 in
-    let? y = rand 10 in
-    let? z = rand 100 in
+    let? w = rand_nat 2 in
+    let? x = rand_nat 2 in
+    let? y = rand_nat 10 in
+    let? z = rand_nat 100 in
     return (w, x, y, z)
   in
   assert_norm (run (init 0) cmp = (0, 1, 4, 75));
   let cmp' =
-    let? w = rand 2 in
-    let? x = rand 2 in
-    let? y = rand 10 in
-    let? z = rand 100 in
+    let? w = rand_nat 2 in
+    let? x = rand_nat 2 in
+    let? y = rand_nat 10 in
+    let? z = rand_nat 100 in
     return (w, x, y, z)
   in
   // The same computation performed with the same seed is the same
   assert_norm (run (init 0) cmp = run (init 0) cmp');
   // The same computation performed with a different seed is different
   assert_norm (run (init 0) cmp =!= run (init 1) cmp')
+
+let _ex_rand_bool =
+  assert_norm (
+    run (init 0) (
+      let? b1 = rand_bool in
+      let? b2 = rand_bool in
+      let? b3 = rand_bool in
+      return (b1, b2, b3)
+    )
+    =
+    (true, false, true)
+  )
+
+let _ex_rand_choice =
+ let l = [1;2;3;4;5] in
+ assert_norm (
+  run (init 0) (
+      let? a = rand_choice l in
+      let? b = rand_choice l in
+      let? c = rand_choice l in
+      let? d = rand_choice l in
+      return (a, b, c, d)
+  )
+  =
+  (4, 5, 5, 1)
+ )
